Revised SHA3 spec and implementation using new loop combinators

code/experimental/sha3/Hacl.Impl.SHA3.fst
@@ -19,6 +19,7 @@ module HS = FStar.HyperStack
 module B = LowStar.Buffer
 module IB = LowStar.ImmutableBuffer
 module LSeq = Lib.Sequence
+module LB = Lib.ByteSequence
 module S = Spec.SHA3
 
 let keccak_rotc = IB.igcmalloc_of_list HyperStack.root rotc_list
@@ -43,7 +44,7 @@ let index = n:size_t{v n < 5}
 
 inline_for_extraction noextract
 val readLane:
-     s:state
+    s:state
   -> x:index
   -> y:index
   -> Stack uint64
@@ -55,7 +56,7 @@ let readLane s x y = s.(x +! size 5 *! y)
 
 inline_for_extraction noextract
 val writeLane:
-     s:state
+    s:state
   -> x:index
   -> y:index
   -> v:uint64
@@ -71,115 +72,84 @@ let rotl (a:uint64) (b:uint32{0 < uint_v b /\ uint_v b < 64}) =
   (a <<. b) |. (a >>. (u32 64 -. b))
 
 inline_for_extraction noextract
-val state_theta_inner_C:
-    #h0:mem
-  -> s:state
-  -> i:index
-  -> _C:lbuffer uint64 5
-  -> Stack unit
-    (requires fun h ->
-      live h s /\ live h _C /\ disjoint _C s /\
-      as_seq h0 s == as_seq h s /\
-      loop_inv h0 h 5 _C (fun h0 -> S.state_theta_inner_C (as_seq h0 s)) (v i))
-    (ensures  fun _ _ h -> live h s /\
-      loop_inv h0 h 5 _C (fun h0 -> S.state_theta_inner_C (as_seq h0 s)) (v i + 1))
-let state_theta_inner_C #h0 s x _C =
-  let h1 = ST.get () in
-  _C.(x) <-
-    readLane s x (size 0) ^.
-    readLane s x (size 1) ^.
-    readLane s x (size 2) ^.
-    readLane s x (size 3) ^.
-    readLane s x (size 4);
-  let h2 = ST.get () in
-  assert (as_seq h2 _C == S.state_theta_inner_C (as_seq h0 s) (v x) (as_seq h1 _C));
-  lemma_repeati_sp #h0 5 (fun h0 -> S.state_theta_inner_C (as_seq h0 s)) (as_seq h0 _C) (v x) (as_seq h1 _C)
-
-inline_for_extraction noextract
 val state_theta0:
-     #h0:mem
-  -> s:state
+    s:state
   -> _C:lbuffer uint64 5
   -> Stack unit
-    (requires fun h ->
-      h0 == h /\ live h s /\ live h _C /\
-      disjoint _C s /\
-      as_seq h0 s == as_seq h s)
-    (ensures  fun _ _ h1 ->
+    (requires fun h -> live h s /\ live h _C /\ disjoint _C s)
+    (ensures  fun h0 _ h1 ->
       modifies (loc_buffer _C) h0 h1 /\
       as_seq h1 _C == S.state_theta0 (as_seq h0 s) (as_seq h0 _C))
-let state_theta0 #h0 s _C =
-  let inv h h1 = live h1 s /\ live h1 _C /\ disjoint s _C /\ as_seq h0 s == as_seq h1 s in
-  loop #h0 (size 5) _C inv (fun h0 -> S.state_theta_inner_C (as_seq h0 s))
-  (fun x ->
-    state_theta_inner_C #h0 s x _C
-  )
-
-inline_for_extraction noextract
-val state_theta_inner_s_inner:
-     #h0:mem
-  -> x:index
-  -> _D:uint64
-  -> y:index
-  -> s:state
-  -> Stack unit
-    (requires fun h -> live h s /\
-      loop_inv h0 h 5 s (fun h0 -> S.state_theta_inner_s_inner (v x) _D) (v y))
-    (requires fun _ _ h ->
-      loop_inv h0 h 5 s (fun h0 -> S.state_theta_inner_s_inner (v x) _D) (v y + 1))
-let state_theta_inner_s_inner #h0 x _D y s =
-  let h1 = ST.get () in
-  writeLane s x y (readLane s x y ^. _D);
-  let h2 = ST.get () in
-  lemma_repeati_sp #h0 5 (fun h0 -> S.state_theta_inner_s_inner (v x) _D) (as_seq h0 s) (v y) (as_seq h1 s)
+let state_theta0 s _C =
+  let a_spec i = LSeq.lseq uint64 5 in 
+  let a_impl = lbuffer uint64 5 in
+  [@ inline_let]
+  let spec h0 = S.state_theta_inner_C (as_seq h0 s) in
+  let h0 = ST.get () in
+  loop h0 (size 5) a_spec a_impl 
+    (fun h i (b:lbuffer uint64 5) -> as_seq h b)
+    (fun i -> loc_buffer _C)
+    spec
+    _C
+    (fun x ->      
+      LSeq.unfold_repeat 5 a_spec (spec h0) (as_seq h0 _C) (v x);
+      _C.(x) <-
+        readLane s x (size 0) ^.
+        readLane s x (size 1) ^.
+        readLane s x (size 2) ^.
+        readLane s x (size 3) ^.
+        readLane s x (size 4)    
+    )
 
 inline_for_extraction noextract
 val state_theta_inner_s:
-     #h0:mem
-  -> _C:lbuffer uint64 5
+    _C:lbuffer uint64 5
   -> x:index
   -> s:state
   -> Stack unit
-    (requires fun h ->
-      live h s /\ live h _C /\ disjoint _C s /\
-      as_seq h0 _C == as_seq h _C /\
-      loop_inv h0 h 5 s (fun h0 -> S.state_theta_inner_s (as_seq h0 _C)) (v x))
-    (ensures  fun _ _ h -> loop_inv h0 h 5 s (fun h0 -> S.state_theta_inner_s (as_seq h0 _C)) (v x + 1))
-let state_theta_inner_s #h0 _C x s =
+    (requires fun h0 -> live h0 s /\ live h0 _C /\ disjoint _C s)
+    (ensures  fun h0 _ h1 -> 
+      modifies (loc_buffer s) h0 h1 /\
+      as_seq h1 s == S.state_theta_inner_s (as_seq h0 _C) (v x) (as_seq h0 s))
+let state_theta_inner_s _C x s =
   let _D = _C.((x +. size 4) %. size 5) ^. rotl _C.((x +. size 1) %. size 5) (u32 1) in
-  let inv h0 h = live h s in
-  let h1 = ST.get () in
-  loop #h1 (size 5) s inv (fun h0 -> S.state_theta_inner_s_inner (v x) _D)
-  (fun y ->
-    state_theta_inner_s_inner #h1 x _D y s
-  );
-  let h2 = ST.get () in
-  assert (as_seq h2 s == LSeq.repeati_sp #5 5 (S.state_theta_inner_s_inner (v x) _D) (as_seq h1 s));
-  lemma_repeati_sp #h0 5 (fun h0 -> S.state_theta_inner_s (as_seq h0 _C)) (as_seq h0 s) (v x) (as_seq h1 s)
+  let a_spec i = S.state in 
+  let refl h i (s:state) : GTot S.state = as_seq h s in
+  let footprint i = loc_buffer s in
+  [@ inline_let]
+  let spec h0 = S.state_theta_inner_s_inner (v x) _D in
+  let h0 = ST.get () in
+  loop h0 (size 5) a_spec state refl footprint spec s
+    (fun y -> 
+      LSeq.unfold_repeat 5 a_spec (spec h0) (as_seq h0 s) (v y);
+      writeLane s x y (readLane s x y ^. _D)
+    )
 
 inline_for_extraction noextract
 val state_theta1:
      s:state
   -> _C:lbuffer uint64 5
   -> Stack unit
-    (requires fun h ->
-      live h s /\ live h _C /\ disjoint _C s)
+    (requires fun h0 -> live h0 s /\ live h0 _C /\ disjoint _C s)
     (ensures  fun h0 _ h1 ->
       modifies (loc_buffer s) h0 h1 /\
       as_seq h1 s == S.state_theta1 (as_seq h0 s) (as_seq h0 _C))
 let state_theta1 s _C =
-  let inv h0 h =
-    live h s /\ live h _C /\ disjoint _C s /\
-    as_seq h0 _C == as_seq h _C in
+  let a_spec i = S.state in
+  let refl h i (s:state) : GTot S.state = as_seq h s in
+  let footprint i = loc_buffer s in
+  [@ inline_let]
+  let spec h0 = S.state_theta_inner_s (as_seq h0 _C) in
   let h0 = ST.get () in
-  loop #h0 (size 5) s inv (fun h0 -> S.state_theta_inner_s (as_seq h0 _C))
+  loop h0 (size 5) a_spec state refl footprint spec s
   (fun x ->
-    state_theta_inner_s #h0 _C x s
+    LSeq.unfold_repeat 5 a_spec (spec h0) (as_seq h0 s) (v x);
+    state_theta_inner_s _C x s
   )
 
 inline_for_extraction noextract
 val state_theta:
-     s:state
+    s:state
   -> Stack unit
     (requires fun h -> live h s)
     (ensures  fun h0 _ h1 ->
@@ -187,9 +157,8 @@ val state_theta:
       as_seq h1 s == S.state_theta (as_seq h0 s))
 let state_theta s =
   push_frame();
-  let _C:lbuffer uint64 5 = create (size 5) (u64 0) in
-  let h0 = ST.get () in
-  state_theta0 #h0 s _C;
+  let _C = create (size 5) (u64 0) in
+  state_theta0 s _C;
   state_theta1 s _C;
   pop_frame()
 
@@ -209,37 +178,33 @@ let rec index_map #a #b f l i =
 
 inline_for_extraction noextract
 val state_pi_rho_inner:
-    #h0:mem
-  -> i:size_t{v i < 24}
+    i:size_t{v i < 24}
   -> current:lbuffer uint64 1
   -> s:state
   -> Stack unit
-    (requires fun h ->
-      live h s /\ live h current /\ disjoint current s /\
-      loop2_inv h0 h 24 current s (fun h0 -> S.state_pi_rho_inner) (v i))
-    (ensures  fun h _ h1 ->
-      loop2_inv h0 h1 24 current s (fun h0 -> S.state_pi_rho_inner) (v i + 1))
-let state_pi_rho_inner #h0 i current s =
+    (requires fun h -> live h s /\ live h current /\ disjoint current s)   
+    (ensures  fun h0 _ h1 ->
+      modifies (loc_union (loc_buffer s) (loc_buffer current)) h0 h1 /\
+      (let c', s' = S.state_pi_rho_inner (v i) (get h0 current 0, as_seq h0 s) in
+      get h1 current 0 == c' /\
+      as_seq h1 s == s'))
+let state_pi_rho_inner i current s =
   let h = ST.get () in
   IB.recall_contents keccak_rotc (Seq.seq_of_list rotc_list);
   IB.recall_contents keccak_piln (Seq.seq_of_list piln_list);
-  let r = IB.index keccak_rotc (Lib.RawIntTypes.size_to_UInt32 i) in
-  //assert (r == LSeq.index S.keccak_rotc (v i));
+  let r  = IB.index keccak_rotc (Lib.RawIntTypes.size_to_UInt32 i) in
   let _Y = IB.index keccak_piln (Lib.RawIntTypes.size_to_UInt32 i) in
   index_map S.sizes_v piln_list (v i);
-  // assert (v _Y == LSeq.index #_ #24 S.keccak_piln (v i));
   let temp = s.(_Y) in
-  let current0:uint64 = current.(size 0) in
+  let current0 = current.(size 0) in
   s.(_Y) <- rotl current0 r;
-  current.(size 0) <- temp;
-  let h1 = ST.get () in
-  lemma_repeati_sp #h0 24 (fun h0 -> S.state_pi_rho_inner) (as_seq h0 current, as_seq h0 s) (v i) (as_seq h current, as_seq h s)
+  current.(size 0) <- temp
 
 #reset-options "--max_fuel 0 --max_ifuel 0 --z3rlimit 50"
 
 inline_for_extraction noextract
 val state_pi_rho:
-     s:state
+    s:state
   -> Stack unit
     (requires fun h -> live h s)
     (ensures  fun h0 _ h1 ->
@@ -248,78 +213,64 @@ val state_pi_rho:
 let state_pi_rho s =
   push_frame();
   let current:lbuffer uint64 1 = create (size 1) (readLane s (size 1) (size 0)) in
+  let a_spec i = tuple2 uint64 S.state in
+  let a_impl = tuple2 (lbuffer uint64 1) state in
+  let refl h i (cs:tuple2 (lbuffer uint64 1) state) : GTot (tuple2 uint64 S.state) = 
+    let current, (s:state) = cs in get h current 0, as_seq h s in
+  let footprint i = loc_union (loc_buffer s) (loc_buffer current) in
+  let spec h0 = S.state_pi_rho_inner in
   let h0 = ST.get () in
-  let inv h0 h1 = live h1 s /\ live h1 current /\ disjoint current s in
-  loop2 #h0 (size 24) current s inv (fun h0 -> S.state_pi_rho_inner)
+  loop h0 (size 24) a_spec a_impl refl footprint spec (current, s)
   (fun i ->
-    state_pi_rho_inner #h0 i current s
+    LSeq.unfold_repeat 24 a_spec (spec h0) (refl h0 0 (current, s)) (v i);
+    state_pi_rho_inner i current s
   );
   pop_frame()
 
 inline_for_extraction noextract
 val state_chi_inner:
-     #h0:mem
-  -> s_pi_rho:state
+    s_pi_rho:state
   -> y:index
   -> x:index
   -> s:state
   -> Stack unit
-    (requires fun h ->
-      live h s_pi_rho /\ live h s /\ disjoint s_pi_rho s /\
-      as_seq h0 s_pi_rho == as_seq h s_pi_rho /\
-      loop_inv h0 h 5 s (fun h0 -> S.state_chi_inner (as_seq h0 s_pi_rho) (v y)) (v x))
-    (ensures  fun h _ h1 ->
-      loop_inv h0 h1 5 s (fun h0 -> S.state_chi_inner (as_seq h0 s_pi_rho) (v y)) (v x + 1))
-let state_chi_inner #h0 s_pi_rho y x s =
-  let h1 = ST.get () in
+    (requires fun h0 -> live h0 s_pi_rho /\ live h0 s /\ disjoint s_pi_rho s)
+    (ensures  fun h0 _ h1 ->
+      modifies (loc_buffer s) h0 h1 /\
+      as_seq h1 s == S.state_chi_inner (as_seq h0 s_pi_rho) (v y) (v x) (as_seq h0 s))
+let state_chi_inner s_pi_rho y x s =
   writeLane s x y
     (readLane s_pi_rho x y ^.
      ((lognot (readLane s_pi_rho ((x +. size 1) %. size 5) y)) &.
-     readLane s_pi_rho ((x +. size 2) %. size 5) y));
-  let h2 = ST.get () in
-  lemma_repeati_sp #h0 5 (fun h0 -> S.state_chi_inner (as_seq h0 s_pi_rho) (v y)) (as_seq h0 s) (v x) (as_seq h1 s)
+     readLane s_pi_rho ((x +. size 2) %. size 5) y))
 
 inline_for_extraction noextract
 val state_chi_inner1:
-    #h0:mem
-  -> s_pi_rho:state
+    s_pi_rho:state
   -> y:index
   -> s:state
   -> Stack unit
-    (requires fun h ->
-      live h s_pi_rho /\ live h s /\ disjoint s_pi_rho s /\
-      as_seq h0 s_pi_rho == as_seq h s_pi_rho /\
-      loop_inv h0 h 5 s (fun h0 -> S.state_chi_inner1 (as_seq h0 s_pi_rho)) (v y))
-    (ensures  fun h _ h1 ->
-      loop_inv h0 h1 5 s (fun h0 -> S.state_chi_inner1 (as_seq h0 s_pi_rho)) (v y + 1))
-let state_chi_inner1 #h0 s_pi_rho y s =
-  let h1 = ST.get () in
-  let inv h0 h1 = live h1 s_pi_rho /\ live h1 s /\ disjoint s_pi_rho s in
-  loop #h1 (size 5) s inv (fun h0 -> S.state_chi_inner (as_seq h0 s_pi_rho) (v y))
-  (fun x ->
-    state_chi_inner #h1 s_pi_rho y x s
-  );
-  let h2 = ST.get () in
-  lemma_repeati_sp #h0 5 (fun h0 -> S.state_chi_inner1 (as_seq h0 s_pi_rho)) (as_seq h0 s) (v y) (as_seq h1 s)
-
-inline_for_extraction noextract
-val copy_s:
-     s0:state
-  -> s1:state
-  -> Stack unit
-    (requires fun h -> live h s0 /\ live h s1 /\ disjoint s0 s1)
+    (requires fun h0 -> live h0 s_pi_rho /\ live h0 s /\ disjoint s_pi_rho s)
     (ensures  fun h0 _ h1 ->
-      modifies (loc_buffer s0) h0 h1 /\
-      as_seq h1 s0 == as_seq h0 s1)
-let copy_s s0 s1 =
+      modifies (loc_buffer s) h0 h1 /\
+      as_seq h1 s == S.state_chi_inner1 (as_seq h0 s_pi_rho) (v y) (as_seq h0 s))
+let state_chi_inner1 s_pi_rho y s =
+  let a_spec i = S.state in
+  let a_impl = state in
+  let refl h i (s:state) : GTot S.state = as_seq h s in
+  let footprint i = loc_buffer s in
+  [@ inline_let]
+  let spec h0 = S.state_chi_inner (as_seq h0 s_pi_rho) (v y) in
   let h0 = ST.get () in
-  update_sub #uint64 #25 s0 (size 0) (size 25) s1;
-  let h1 = ST.get () in
-  LSeq.eq_intro (LSeq.sub #_ #25 (as_seq h1 s0) 0 25) (LSeq.sub #_ #25 (as_seq h0 s1) 0 25)
+  loop h0 (size 5) a_spec a_impl refl footprint spec s
+  (fun x ->
+    LSeq.unfold_repeat 5 a_spec (spec h0) (refl h0 0 s) (v x);
+    state_chi_inner s_pi_rho y x s
+  )
 
 inline_for_extraction noextract
 val state_chi:
-     s:state
+    s:state
   -> Stack unit
     (requires fun h -> live h s)
     (ensures  fun h0 _ h1 ->
@@ -327,19 +278,25 @@ val state_chi:
       as_seq h1 s == S.state_chi (as_seq h0 s))
 let state_chi s =
   push_frame ();
-  let s_pi_rho:state = create (size 25) (u64 0) in
-  copy_s s_pi_rho s;
+  let s_pi_rho: state = create (size 25) (u64 0) in
+  copy s_pi_rho (size 25) s;
+  let a_spec i = S.state in
+  let a_impl = state in
+  let refl h i (s:state) : GTot S.state = as_seq h s in
+  let footprint i = loc_buffer s in
+  [@ inline_let]
+  let spec h0 = S.state_chi_inner1 (as_seq h0 s_pi_rho) in
   let h0 = ST.get () in
-  let inv h0 h1 = live h1 s_pi_rho /\ live h1 s /\ disjoint s_pi_rho s in
-  loop #h0 (size 5) s inv (fun h0 -> S.state_chi_inner1 (as_seq h0 s_pi_rho))
+  loop h0 (size 5) a_spec a_impl refl footprint spec s
   (fun y ->
-    state_chi_inner1 #h0 s_pi_rho y s
+    LSeq.unfold_repeat 5 a_spec (spec h0) (refl h0 0 s) (v y);
+    state_chi_inner1 s_pi_rho y s
   );
-  pop_frame ()
-
+  pop_frame()
+ 
 inline_for_extraction noextract
 val state_iota:
-     s:state
+    s:state
   -> round:size_t{v round < 24}
   -> Stack unit
     (requires fun h -> live h s)
@@ -351,60 +308,32 @@ let state_iota s round =
   writeLane s (size 0) (size 0) (readLane s (size 0) (size 0) ^.
     (IB.index keccak_rndc (Lib.RawIntTypes.size_to_UInt32 round)))
 
-val state_permute1:
-     #h0:mem
-  -> round:size_t{v round < 24}
-  -> s:state
-  -> Stack unit
-    (requires fun h1 -> live h1 s /\ modifies (loc_buffer s) h0 h1 /\
-      as_seq h1 s == LSeq.repeati_sp #24 (v round) S.state_permute1 (as_seq h0 s))
-    (ensures  fun _ _ h1 ->  modifies (loc_buffer s) h0 h1 /\
-      as_seq h1 s == LSeq.repeati_sp #24 (v round + 1) S.state_permute1 (as_seq h0 s))
-let state_permute1 #h0 round s =
-  let h1 = ST.get () in
-  state_theta s;
-  state_pi_rho s;
-  state_chi s;
-  state_iota s round;
-  let h2 = ST.get () in
-  lemma_repeati_sp #h0 24 (fun h0 -> S.state_permute1) (as_seq h0 s) (v round) (as_seq h1 s)
-
 val state_permute:
-     s:state
+    s:state
   -> Stack unit
     (requires fun h -> live h s)
     (ensures  fun h0 _ h1 ->
       modifies (loc_buffer s) h0 h1 /\
       as_seq h1 s == S.state_permute (as_seq h0 s))
 let state_permute s =
+  let a_spec i = S.state in
+  let a_impl = state in
+  let refl h i (s:state) : GTot S.state = as_seq h s in
+  let footprint i = loc_buffer s in
+  [@ inline_let]
+  let spec h0 = S.state_permute1 in
   let h0 = ST.get () in
-  let inv h0 h1 = live h1 s in
-  loop #h0 (size 24) s inv (fun h0 -> S.state_permute1)
-  (fun i ->
-    state_permute1 #h0 i s
+  loop h0 (size 24) a_spec a_impl refl footprint spec s
+  (fun round ->
+    LSeq.unfold_repeat 24 a_spec (spec h0) (refl h0 0 s) (v round);
+    state_theta s;
+    state_pi_rho s;
+    state_chi s;
+    state_iota s round
   )
 
-inline_for_extraction noextract
-val loadState_inner:
-     #h0:mem
-  -> block:lbytes 200
-  -> j:size_t{v j < 25}
-  -> s:state
-  -> Stack unit
-    (requires fun h ->
-      live h block /\ live h s /\ disjoint block s /\
-      as_seq h0 block == as_seq h block /\
-      loop_inv h0 h 25 s (fun h0 -> S.loadState_inner (as_seq h0 block)) (v j))
-    (ensures  fun h _ h1 ->
-      loop_inv h0 h1 25 s (fun h0 -> S.loadState_inner (as_seq h0 block)) (v j + 1))
-let loadState_inner #h0 block j s =
-  let h1 = ST.get () in
-  s.(j) <- s.(j) ^. uint_from_bytes_le #U64 (sub #_ #200 #8 block (j *! size 8) (size 8));
-  let h2 = ST.get () in
-  lemma_repeati_sp #h0 25 (fun h0 -> S.loadState_inner (as_seq h0 block)) (as_seq h0 s) (v j) (as_seq h1 s)
-
 val loadState:
-     rateInBytes:size_t{v rateInBytes <= 200}
+    rateInBytes:size_t{v rateInBytes <= 200}
   -> input:lbytes (v rateInBytes)
   -> s:state
   -> Stack unit
@@ -417,65 +346,76 @@ let loadState rateInBytes input s =
   push_frame();
   let block:lbytes 200 = create (size 200) (u8 0) in
   update_sub block (size 0) rateInBytes input;
+  let a_spec i = S.state in
+  let a_impl = state in
+  let refl h i (s:state) : GTot S.state = as_seq h s in
+  let footprint i = loc_buffer s in
+  [@ inline_let]
+  let spec h0 = S.loadState_inner (as_seq h0 block) in
   let h0 = ST.get () in
-  let inv h0 h1 =
-    live h1 block /\ live h1 s /\ disjoint block s /\
-    as_seq h0 block == as_seq h1 block in
-  loop #h0 (size 25) s inv (fun h0 -> S.loadState_inner (as_seq h0 block))
-  (fun i ->
-    loadState_inner #h0 block i s
+  loop h0 (size 25) a_spec a_impl refl footprint spec s
+  (fun j ->
+    LSeq.unfold_repeat 25 a_spec (spec h0) (refl h0 0 s) (v j);
+    s.(j) <- s.(j) ^. uint_from_bytes_le #U64 (sub #_ #200 #8 block (j *! size 8) (size 8))
   );
   pop_frame ()
 
 inline_for_extraction noextract
 val storeState_inner:
-     #h0:mem
-  -> s:state
+    s:state
   -> j:size_t{v j < 25}
   -> block:lbytes 200
   -> Stack unit
-    (requires fun h ->
-      live h s /\ live h block /\ disjoint s block /\
-      as_seq h0 s == as_seq h s /\
-      loop_inv h0 h 25 block (fun h0 -> S.storeState_inner (as_seq h0 s)) (v j))
-    (ensures  fun h _ h1 ->
-      loop_inv h0 h1 25 block (fun h0 -> S.storeState_inner (as_seq h0 s)) (v j + 1))
-let storeState_inner #h0 s j block =
+    (requires fun h0 -> live h0 s /\ live h0 block /\ disjoint s block)
+    (ensures  fun h0 _ h1 ->
+      modifies (loc_buffer block) h0 h1 /\
+      as_seq h1 block == S.storeState_inner (as_seq h0 s) (v j) (as_seq h0 block))
+let storeState_inner s j block =
   let h1 = ST.get () in
   let tmp = sub block (j *! size 8) (size 8) in
   uint_to_bytes_le tmp s.(j);
   let h2 = ST.get () in
-  assert (v j * 8 < 200);
-  modifies_buffer_elim (sub #uint8 #200 #(v j * 8) block (size 0) (j *! size 8)) (loc_buffer tmp) h1 h2;
-  modifies_buffer_elim (sub #uint8 #200 #(200 - v j * 8 - 8) block (j *! size 8 +! size 8) (size 200 -! j *! size 8 -! size 8)) (loc_buffer tmp) h1 h2;
-  S.lemma_update_store (as_seq h1 s) (v j) (as_seq h1 block) (as_seq h2 block);
-  assert (as_seq h2 block == S.storeState_inner (as_seq h1 s) (v j) (as_seq h1 block));
-  lemma_repeati_sp #h0 25 (fun h0 -> S.storeState_inner (as_seq h0 s)) (as_seq h0 block) (v j) (as_seq h1 block)
+  modifies_buffer_elim 
+    (sub #_ #_ #(v j * 8) block (size 0) (j *! size 8)) (loc_buffer tmp) h1 h2;
+  modifies_buffer_elim 
+    (sub #_ #_ #(200 - v j * 8 - 8) block (j *! size 8 +! size 8) (size 200 -! j *! size 8 -! size 8)) (loc_buffer tmp) h1 h2;
+  Seq.lemma_eq_intro (as_seq h2 block) 
+    (S.storeState_inner (as_seq h1 s) (v j) (as_seq h1 block))
 
 val storeState:
-     rateInBytes:size_t{v rateInBytes <= 200}
+    rateInBytes:size_t{v rateInBytes <= 200}
   -> s:state
   -> res:lbytes (v rateInBytes)
   -> Stack unit
-    (requires fun h -> live h s /\ live h res /\ disjoint s res)
+    (requires fun h0 -> live h0 s /\ live h0 res /\ disjoint s res)
     (ensures  fun h0 _ h1 ->
       modifies (loc_buffer res) h0 h1 /\
       as_seq h1 res == S.storeState (v rateInBytes) (as_seq h0 s))
 let storeState rateInBytes s res =
+  let h = ST.get() in
   push_frame();
   let block:lbytes 200 = create (size 200) (u8 0) in
+  let a_spec (i:size_nat{i <= 25}) = LB.lbytes 200 in
+  let a_impl = lbytes 200 in
+  let refl h i (block:lbytes 200) : GTot (a_spec i) = as_seq h block in
+  let footprint i = loc_buffer block in
+  [@ inline_let]
+  let spec h0 = S.storeState_inner (as_seq h0 s) in
   let h0 = ST.get () in
-  let inv h0 h = live h s /\ live h block /\ disjoint s block in
-  loop #h0 (size 25) block inv (fun h0 -> S.storeState_inner (as_seq h0 s))
+  loop h0 (size 25) a_spec a_impl refl footprint spec block
   (fun j ->
-    storeState_inner #h0 s j block
+    LSeq.unfold_repeat 25 a_spec (spec h0) (refl h0 0 block) (v j);
+    storeState_inner s j block
   );
   update_sub res (size 0) rateInBytes (sub block (size 0) rateInBytes);
   pop_frame()
+  
+
+#reset-options "--z3rlimit 50 --max_fuel 0 --max_ifuel 0 --using_facts_from '* -FStar.Seq'"
 
 inline_for_extraction noextract
 val absorb_last:
-     s:state
+    s:state
   -> rateInBytes:size_t{v rateInBytes > 0 /\ v rateInBytes <= 200}
   -> inputByteLen:size_t
   -> input:lbytes (v inputByteLen)
@@ -490,23 +430,26 @@ let absorb_last s rateInBytes inputByteLen input delimitedSuffix =
   push_frame ();
   let lastBlock = create rateInBytes (u8 0) in
   let rem = inputByteLen %. rateInBytes in
-  assert (v rem == v inputByteLen % v rateInBytes);
   let last = sub input (inputByteLen -. rem) rem in
   let h0 = ST.get () in
   update_sub #uint8 #(v rateInBytes) lastBlock (size 0) rem last;
-  let h1 = ST.get () in
-  assert (as_seq h1 lastBlock == LSeq.update_sub #uint8 #(v rateInBytes) (as_seq h0 lastBlock) 0 (v rem) (as_seq h0 last));
+  assert (v rem < v rateInBytes);
   lastBlock.(rem) <- delimitedSuffix;
-  let h2 = ST.get () in
-  assert (as_seq h2 lastBlock == LSeq.upd #uint8 #(v rateInBytes) (as_seq h1 lastBlock) (v rem) delimitedSuffix);
   loadState rateInBytes lastBlock s;
-  let h3 = ST.get () in
-  assert (as_seq h3 s == S.loadState (v rateInBytes) (as_seq h2 lastBlock) (as_seq h2 s));
-  pop_frame ()
+  pop_frame();
+  // TODO: this seems unnecessary
+  let h1 = ST.get () in
+  assert (as_seq h1 s == 
+    (let lastBlock = LSeq.create (v rateInBytes) (u8 0) in
+     let rem = v inputByteLen % v rateInBytes in
+     let last: LSeq.lseq uint8 rem = LSeq.sub #_ #(v inputByteLen) (as_seq h0 input) (v inputByteLen - rem) rem in
+     let lastBlock = LSeq.update_sub lastBlock 0 rem last in
+     let lastBlock = Lib.Sequence.(lastBlock.[rem] <- delimitedSuffix) in
+     S.loadState (v rateInBytes) lastBlock (as_seq h0 s)))
 
 inline_for_extraction noextract
 val absorb_next:
-     s:state
+    s:state
   -> rateInBytes:size_t{v rateInBytes > 0 /\ v rateInBytes <= 200}
   -> Stack unit
     (requires fun h -> live h s)
@@ -521,44 +464,41 @@ let absorb_next s rateInBytes =
   state_permute s;
   pop_frame ()
 
+private
+val lemma_rateInBytes:
+    inputByteLen:size_nat
+  -> rateInBytes:size_nat{0 < rateInBytes /\ rateInBytes <= 200}
+  -> i:size_nat{i < inputByteLen / rateInBytes}
+  -> Lemma (i * rateInBytes + rateInBytes <= inputByteLen)
+let lemma_rateInBytes _ _ _ = ()
+
 inline_for_extraction noextract
 val absorb_inner:
-     #h0:mem
-  -> rateInBytes:size_t{v rateInBytes > 0 /\ v rateInBytes <= 200}
+    rateInBytes:size_t{0 < v rateInBytes /\ v rateInBytes <= 200}
   -> inputByteLen:size_t
   -> input:lbytes (v inputByteLen)
   -> i:size_t{v i < v inputByteLen / v rateInBytes}
   -> s:state
   -> Stack unit
-    (requires fun h ->
-      live h s /\ live h input /\ disjoint s input /\
-      as_seq h0 input == as_seq h input /\
-      modifies (loc_buffer s) h0 h /\
-      as_seq h s ==
-      LSeq.repeati_sp #(v inputByteLen / v rateInBytes) (v i)
-	(S.absorb_inner (v rateInBytes) (v inputByteLen) (as_seq h0 input)) (as_seq h0 s))
-    (ensures  fun h _ h1 ->
+    (requires fun h0 -> live h0 s /\ live h0 input /\ disjoint s input)
+    (ensures  fun h0 _ h1 ->
       modifies (loc_buffer s) h0 h1 /\
-      as_seq h1 s ==
-      LSeq.repeati_sp #(v inputByteLen / v rateInBytes) (v i + 1)
-	(S.absorb_inner (v rateInBytes) (v inputByteLen) (as_seq h0 input)) (as_seq h0 s))
-let absorb_inner #h0 rateInBytes inputByteLen input i s =
-  let h1 = ST.get () in
-  S.lemma_rateInBytes (v inputByteLen) (v rateInBytes) (v i);
-  loadState rateInBytes (sub #_ #(v inputByteLen) #(v rateInBytes) input (i *! rateInBytes) rateInBytes) s;
-  state_permute s;
-  let h2 = ST.get () in
-  lemma_repeati_sp #h0 (v inputByteLen / v rateInBytes)
-    (fun h0 -> S.absorb_inner (v rateInBytes) (v inputByteLen) (as_seq h0 input)) (as_seq h0 s) (v i) (as_seq h1 s)
+      as_seq h1 s == 
+      S.absorb_inner (v rateInBytes) (v inputByteLen) (as_seq h0 input) (v i) (as_seq h0 s))
+let absorb_inner rateInBytes inputByteLen input i s =
+  lemma_rateInBytes (v inputByteLen) (v rateInBytes) (v i);
+  loadState rateInBytes 
+    (sub #_ #(v inputByteLen) #(v rateInBytes) input (i *! rateInBytes) rateInBytes) s;
+  state_permute s
 
 val absorb:
-     s:state
-  -> rateInBytes:size_t{v rateInBytes > 0 /\ v rateInBytes <= 200}
+    s:state
+  -> rateInBytes:size_t{0 < v rateInBytes /\ v rateInBytes <= 200}
   -> inputByteLen:size_t
   -> input:lbytes (v inputByteLen)
   -> delimitedSuffix:uint8
   -> Stack unit
-    (requires fun h -> live h s /\ live h input /\ disjoint s input)
+    (requires fun h0 -> live h0 s /\ live h0 input /\ disjoint s input)
     (ensures  fun h0 _ h1 ->
       modifies (loc_buffer s) h0 h1 /\
       as_seq h1 s ==
@@ -567,93 +507,123 @@ let absorb s rateInBytes inputByteLen input delimitedSuffix =
   let open Lib.RawIntTypes in
   let n = inputByteLen /. rateInBytes in
   let rem = inputByteLen %. rateInBytes in
+  let a_spec (i:size_nat{i <= v inputByteLen / v rateInBytes}) = S.state in
+  let a_impl = state in
+  let refl h i (s:state) : GTot (a_spec i) = as_seq h s in
+  let footprint i = loc_buffer s in
+  [@ inline_let]
+  let spec h0 = S.absorb_inner (v rateInBytes) (v inputByteLen) (as_seq h0 input) in
   let h0 = ST.get () in
-  let inv h0 h =
-    live h s /\ live h input /\ disjoint s input /\
-    as_seq h0 input == as_seq h input in
-  loop #h0 n s inv (fun h0 -> S.absorb_inner (v rateInBytes) (v inputByteLen) (as_seq h0 input))
+  loop h0 n a_spec a_impl refl footprint spec s
   (fun i ->
-    absorb_inner #h0 rateInBytes inputByteLen input i s
+    LSeq.unfold_repeat (v n) a_spec (spec h0) (refl h0 0 s) (v i);
+    absorb_inner rateInBytes inputByteLen input i s
   );
   absorb_last s rateInBytes inputByteLen input delimitedSuffix;
   (if (not (u8_to_UInt8 (delimitedSuffix &. u8 0x80) = 0uy) && (size_to_UInt32 rem = size_to_UInt32 (rateInBytes -. size 1)))
   then state_permute s);
-  absorb_next s rateInBytes
+  absorb_next s rateInBytes;
+  let h1 = ST.get () in
+  // TODO: Figure out why S.absorb doesn't unfold
+  let foo (p:Type0) 
+    (pp:squash (norm [delta_only ["Spec.SHA3.absorb"]] p)) : squash p = pp
+  in
+  foo (
+    as_seq h1 s ==
+    S.absorb (as_seq h0 s) (v rateInBytes) (v inputByteLen) (as_seq h0 input) delimitedSuffix) ()
+
+#reset-options "--z3rlimit 50 --max_fuel 0 --max_ifuel 0 --using_facts_from '*'"
+
+val lemma_update_squeeze:
+    rateInBytes:size_nat{0 < rateInBytes /\ rateInBytes <= 200}
+  -> outputByteLen:size_nat
+  -> i:size_nat{i < outputByteLen / rateInBytes}
+  -> s:S.state
+  -> o:LB.lbytes (i * rateInBytes)
+  -> o1:LB.lbytes (i * rateInBytes + rateInBytes)
+  -> Lemma
+    (requires
+      LSeq.sub o1 0 (i * rateInBytes) == LSeq.sub o 0 (i * rateInBytes) /\
+      LSeq.sub o1 (i * rateInBytes) rateInBytes == S.storeState rateInBytes s)
+    (ensures o1 == snd (S.squeeze_inner rateInBytes outputByteLen i (s, o)))
+let lemma_update_squeeze rateInBytes outputByteLen i s o o1 =
+  Seq.lemma_split (LSeq.sub o1 0 (i * rateInBytes + rateInBytes)) (i * rateInBytes)
 
 inline_for_extraction noextract
 val squeeze_inner:
-     #h0:mem
-  -> rateInBytes:size_t{v rateInBytes > 0 /\ v rateInBytes <= 200}
+    rateInBytes:size_t{0 < v rateInBytes /\ v rateInBytes <= 200}
   -> outputByteLen:size_t
   -> i:size_t{v i < v outputByteLen / v rateInBytes}
   -> s:state
   -> output:lbytes (v outputByteLen)
   -> Stack unit
-    (requires fun h ->
-      live h s /\ live h output /\ disjoint s output /\
-      loop2_inv h0 h (v outputByteLen / v rateInBytes) s output
-        (fun h0 -> S.squeeze_inner (v rateInBytes) (v outputByteLen)) (v i))
-    (ensures  fun h _ h1 ->
-      loop2_inv h0 h1 (v outputByteLen / v rateInBytes) s output
-        (fun h0 -> S.squeeze_inner (v rateInBytes) (v outputByteLen)) (v i + 1))
-let squeeze_inner #h0 rateInBytes outputByteLen i s output =
-  S.lemma_rateInBytes (v outputByteLen) (v rateInBytes) (v i);
-  let h1 = ST.get () in
-  let tmp = sub output (i *! rateInBytes) rateInBytes in
-  storeState rateInBytes s tmp;
-  let h2 = ST.get () in
-  modifies_buffer_elim (sub #uint8 #(v outputByteLen) #(v i * v rateInBytes) output (size 0) (i *! rateInBytes)) (loc_buffer tmp) h1 h2;
-  modifies_buffer_elim (sub #uint8 #(v outputByteLen) #(v outputByteLen - v i * v rateInBytes - v rateInBytes)
-    output (i *! rateInBytes +! rateInBytes) (outputByteLen -! i *! rateInBytes -! rateInBytes)) (loc_buffer tmp) h1 h2;
-  S.lemma_update_squeeze (v rateInBytes) (v outputByteLen) (v i) (as_seq h1 s) (as_seq h1 output) (as_seq h2 output);
-  state_permute s;
-  lemma_repeati_sp #h0 (v outputByteLen / v rateInBytes) (fun h0 -> S.squeeze_inner (v rateInBytes) (v outputByteLen))
-    (as_seq h0 s, as_seq h0 output) (v i) (as_seq h1 s, as_seq h1 output)
-
-inline_for_extraction noextract
-val squeeze_rem:
-     s:state
-  -> rateInBytes:size_t{v rateInBytes > 0 /\ v rateInBytes <= 200}
-  -> outputByteLen:size_t
-  -> output:lbytes (v outputByteLen)
-  -> Stack unit
-    (requires fun h -> live h s /\ live h output /\ disjoint s output)
+    (requires fun h0 -> live h0 s /\ live h0 output /\ disjoint s output)
     (ensures  fun h0 _ h1 ->
-      modifies (loc_buffer output) h0 h1 /\
-      as_seq h1 output ==
-      S.squeeze_rem (as_seq h0 s) (v rateInBytes) (v outputByteLen) (as_seq h0 output))
-let squeeze_rem s rateInBytes outputByteLen output =
-  let remOut = outputByteLen %. rateInBytes in
+      lemma_rateInBytes (v outputByteLen) (v rateInBytes) (v i);
+      modifies (loc_union (loc_buffer s) (loc_buffer output)) h0 h1 /\
+ //       (loc_buffer (gsub #_ #_ #(v rateInBytes) output (i *! rateInBytes) rateInBytes))) h0 h1 /\
+      (let o = as_seq h0 (gsub #_ #_ #(v i * v rateInBytes) output (size 0) (i *! rateInBytes)) in
+       let s', output' = 
+         S.squeeze_inner (v rateInBytes) (v outputByteLen) (v i) (as_seq h0 s, o) in 
+       as_seq h1 s == s' /\
+       as_seq h1 (gsub #_ #_ #((v i + 1) * v rateInBytes) output (size 0) ((i +! size 1) *! rateInBytes)) == output'))
+let squeeze_inner rateInBytes outputByteLen i s output =
+  lemma_rateInBytes (v outputByteLen) (v rateInBytes) (v i);
+  let h0 = ST.get () in
+  storeState rateInBytes s (sub output (i *! rateInBytes) rateInBytes);
   let h1 = ST.get () in
-  let tmp = sub output (outputByteLen -. remOut) remOut in
-  storeState remOut s tmp;
-  let h2 = ST.get () in
-  modifies_buffer_elim (sub #uint8 #(v outputByteLen) #(v outputByteLen - v remOut) output (size 0) (outputByteLen -! remOut)) (loc_buffer tmp) h1 h2;
-  S.lemma_update_squeeze_rem (as_seq h1 s) (v rateInBytes) (v outputByteLen) (as_seq h1 output) (as_seq h2 output)
+  state_permute s;
+  let o = as_seq h0 (gsub #_ #_ #(v i * v rateInBytes) output (size 0) (i *! rateInBytes)) in
+  let o' = as_seq h1 (gsub #_ #_  #((v i + 1) * v rateInBytes) output (size 0) ((i +! size 1) *! rateInBytes)) in
+  lemma_update_squeeze (v rateInBytes) (v outputByteLen) (v i) (as_seq h1 s) o o'
+
+#set-options "--max_ifuel 1"
 
 val squeeze:
-     s:state
-  -> rateInBytes:size_t{v rateInBytes > 0 /\ v rateInBytes <= 200}
+    s:state
+  -> rateInBytes:size_t{0 < v rateInBytes /\ v rateInBytes <= 200}
   -> outputByteLen:size_t
   -> output:lbytes (v outputByteLen)
   -> Stack unit
-    (requires fun h -> live h s /\ live h output /\ disjoint s output)
+    (requires fun h0 -> live h0 s /\ live h0 output /\ disjoint s output)
     (ensures  fun h0 _ h1 ->
       modifies (loc_union (loc_buffer s) (loc_buffer output)) h0 h1 /\
-      as_seq h1 output ==
-      S.squeeze (as_seq h0 s) (v rateInBytes) (v outputByteLen) (as_seq h0 output))
+      as_seq h1 output == 
+      S.squeeze (as_seq h0 s) (v rateInBytes) (v outputByteLen))
 let squeeze s rateInBytes outputByteLen output =
+  let h0 = ST.get() in
+  assert_norm (norm [delta] S.squeeze (as_seq h0 s) (v rateInBytes) (v outputByteLen) ==
+    S.squeeze (as_seq h0 s) (v rateInBytes) (v outputByteLen));
   let outBlocks = outputByteLen /. rateInBytes in
+  let remOut = outputByteLen %. rateInBytes in
+  let tmp = sub output (outputByteLen -. remOut) remOut in  
+  let a_spec (i:size_nat{i <= v outputByteLen / v rateInBytes}) =
+    tuple2 S.state (LB.lbytes (i * v rateInBytes)) in
+  let a_impl = tuple2 state (lbytes (v outputByteLen)) in
+  let refl h (i:size_nat{i <= v outBlocks}) (so:tuple2 state (lbytes (v outputByteLen))) :
+    GTot (tuple2 S.state (LB.lbytes (i * v rateInBytes))) =
+    assert (i * v rateInBytes <= v outputByteLen);
+    let s, output = so in
+    as_seq h s, 
+    as_seq h (gsub #_ #_ #(i * v rateInBytes) output (size 0) (size i *! rateInBytes))
+  in
+  let footprint i = loc_union (loc_buffer s) (loc_buffer output) in
+  let spec h0: i:size_nat{i < v outBlocks} -> so:a_spec i -> a_spec (i + 1) = 
+    S.squeeze_inner (v rateInBytes) (v outputByteLen) in
   let h0 = ST.get () in
-  let inv h0 h = live h s /\ live h output /\ disjoint s output in
-  loop2 #h0 outBlocks s output inv (fun h0 -> S.squeeze_inner (v rateInBytes) (v outputByteLen))
+  loop h0 outBlocks a_spec a_impl refl footprint spec (s, output)
   (fun i ->
-    squeeze_inner #h0 rateInBytes outputByteLen i s output
-  );
-  squeeze_rem s rateInBytes outputByteLen output
-
+    LSeq.unfold_repeat (v outBlocks) a_spec (spec h0) (refl h0 0 (s, output)) (v i);    
+    squeeze_inner rateInBytes outputByteLen i s output
+  ); 
+  storeState remOut s tmp;
+  let h1 = ST.get() in
+  Seq.lemma_split (as_seq h1 output) (v outputByteLen - v remOut);
+  Seq.lemma_eq_intro (LSeq.create 0 (u8 0))
+    (as_seq h0 (gsub #_ #_ #0 output (size 0) (size 0)))
+  
 val keccak:
-     rate:size_t{v rate % 8 == 0 /\ v rate / 8 > 0 /\ v rate <= 1600}
+    rate:size_t{v rate % 8 == 0 /\ v rate / 8 > 0 /\ v rate <= 1600}
   -> capacity:size_t{v capacity + v rate == 1600}
   -> inputByteLen:size_t
   -> input:lbytes (v inputByteLen)
@@ -665,7 +635,7 @@ val keccak:
     (ensures  fun h0 _ h1 ->
       modifies (loc_buffer output) h0 h1 /\
       as_seq h1 output ==
-      S.keccak (v rate) (v capacity) (v inputByteLen) (as_seq h0 input) delimitedSuffix (v outputByteLen) (as_seq h0 output))
+      S.keccak (v rate) (v capacity) (v inputByteLen) (as_seq h0 input) delimitedSuffix (v outputByteLen))
 let keccak rate capacity inputByteLen input delimitedSuffix outputByteLen output =
   push_frame();
   let rateInBytes = rate /. size 8 in
